2)f(x)=\dfrac{(x^2-2)\sin^2x}{x+1}
\\f'(x)=\dfrac{((x^2-2)\sin^2x)'(x+1)-(x^2-2)\sin^2x(x+1)'}{(x+1)^2}
\\f'(x)=\dfrac{((x^2-2)'\sin^2x+(x^2-2)(\sin^2x)')(x+1)-(x^2-2)\sin^2x\cancel{(x'+1')}}{(x+1)^2}
\\f'(x)=\dfrac{(((x^2)'-\cancel{2'})\sin^2x+(x^2-2)2\sin x(\sin x)')(x+1)-(x^2-2)\sin^2x\cancel{(x'+1')}}{(x+1)^2}
\\f'(x)=\dfrac{(2x\sin^2x+2(x^2-2)\sin x(-\cos x))(x+1)-(x^2-2)\sin^2x}{(x+1)^2}
\\f'(x)=\dfrac{2\sin x(x\sin x+(x^2-2)(-\cos x))(x+1)-(x^2-2)\sin^2x}{(x+1)^2}
\\f'(x)=\dfrac{2\sin x(x\sin x+(x^2-2)(-\cos x))(x+1)-(x^2-2)\sin^2x}{(x+1)^2}