1)f(x)=\dfrac{(6x^2-x)^4\ln x}{x^2+1}
\\f'(x)=\dfrac{\left((6x^2-x)^4\ln x\right)'(x^2+1)-(6x^2-x)^4\ln x(x^2+1)'}{(x^2+1)^2}
\\f'(x)=\dfrac{\left(((6x^2-x)^4)'\ln x+(6x^2-x)^4\ln x'\right)(x^2+1)-(6x^2-x)^4\ln x((x^2)'+1')}{(x^2+1)^2}
\\f'(x)=\dfrac{\left(4(6x^2-x)^3(6x^2-x)'\ln x+\dfrac{(6x^2-x)^4}x\right)(x^2+1)-2x(6x^2-x)^4\ln x}{(x^2+1)^2}
\\f'(x)=\dfrac{\left(4x^3(6x-1)^3((6x^2)'-x')\ln x+\dfrac{x^4(6x-1)^4}x\right)(x^2+1)-2x^5(6x-1)^4\ln x}{(x^2+1)^2}
\\f'(x)=\dfrac{x^3(6x-1)^3(4(12x-1)\ln x+(6x-1))(x^2+1)-2x^5(6x-1)^4\ln x}{(x^2+1)^2}
\\f'(x)=\dfrac{x^3(6x-1)^3(4(12x-1)\ln x+(6x-1)(x^2+1)-2x^2(6x-1)\ln x)}{(x^2+1)^2}