\\10) f_{(x)}=\dfrac{2x}{x+1}
\\\\f'_{(x)}=\lim_{\Delta x\rightarrow0}\dfrac{\dfrac{2(x+\Delta x)}{x+\Delta x+1}-\dfrac{2x}{x+1}}{\Delta x}
\\\\f'_{(x)}=\lim_{\Delta x\rightarrow0}\dfrac{\dfrac{2x+2\Delta x}{x+\Delta x+1}-\dfrac{2x}{x+1}}{\Delta x}
\\\\f'_{(x)}=\lim_{\Delta x\rightarrow0}\dfrac{\dfrac{(2x+2\Delta x)(x+1)-2x(x+\Delta x+1)}{(x+\Delta x+1)(x+1)}}{\Delta x}
\\\\f'_{(x)}=\lim_{\Delta x\rightarrow0}\dfrac{\cancel{2x^2}+\cancel{2x\Delta x}+\cancel{2x}+2\Delta x-\cancel{2x^2}-\cancel{2x\Delta x}-\cancel{2x}}{\Delta x(x+\Delta x+1)(x+1)}
\\\\f'_{(x)}=\lim_{\Delta x\rightarrow0}\dfrac{2\cancel{\Delta x}}{\cancel{\Delta x}(x+\Delta x+1)(x+1)}
\\\\f'_{(x)}=\dfrac{2}{(x+\cancel0+1)(x+1)}
\\\\f'_{(x)}=\dfrac{2}{(x+1)^2}