\\6) f_{(x)}=\dfrac{x}{x^2-1}
\\\\f'_{(x)}=\lim_{\Delta x\rightarrow 0}\dfrac{\dfrac{x+\Delta x}{(x+\Delta x)^2-1}-\dfrac{x}{x^2-1}}{\Delta x}=
\\\\f'_{(x)}=\lim_{\Delta x\rightarrow 0}\dfrac{\dfrac{(x+\Delta x)(x^2-1)-x((x+\Delta x)^2-1)}{((x+\Delta x)^2-1)(x^2-1)}}{\Delta x}=
\\\\f'_{(x)}=\lim_{\Delta x\rightarrow 0}\dfrac{\cancel{x^3}+x^2\Delta x\cancel{-x}-\Delta x\cancel{-x^3}-2x^2\Delta x-x\Delta x^2+\cancel{x}}{\Delta x((x+\Delta x)^2-1)(x^2-1)}=
\\\\f'_{(x)}=\lim_{\Delta x\rightarrow 0}\dfrac{\cancel{\Delta x}(-1-x^2-x\Delta x)}{\cancel{\Delta x}((x+\Delta x)^2-1)(x^2-1)}=
\\\\f'_{(x)}=\dfrac{-1-x^2-\cancel 0}{((x+\cancel 0)^2-1)(x^2-1)}=
\\\\f'_{(x)}=\dfrac{-x^2-1}{(x^2-1)^2}=\dfrac{-(x^2+1)}{(x^2-1)^2}