1)f_{(x)}=(x+1)^2=
\\f'_{(x)}=\lim_{\Delta x\rightarrow0}\dfrac{((x+\Delta x)+1)^2-(x+1)^2}{\Delta x}=
\\f'_{(x)}=\lim_{\Delta x\rightarrow0}\dfrac{(x+\Delta x+1)^2-(x+1)^2}{\Delta x}=
\\f'_{(x)}=\lim_{\Delta x\rightarrow0}\dfrac{(x^2+\Delta x^2+1+2x\Delta x+2x+2\Delta x)-(x^2+2x+1)}{\Delta x}=
\\f'_{(x)}=\lim_{\Delta x\rightarrow0}\dfrac{x^2+\Delta x^2+1+2x\Delta x+2x+2\Delta x-x^2-2x-1}{\Delta x}=
\\f'_{(x)}=\lim_{\Delta x\rightarrow0}\dfrac{\Delta x^2+2x\Delta x+2\Delta x}{\Delta x}=
\\f'_{(x)}=\lim_{\Delta x\rightarrow0}\dfrac{\Delta x(\Delta x+2x+2)}{\Delta x}=
\\f'_{(x)}=\lim_{\Delta x\rightarrow0}\Delta x+2x+2=
\\f'_{(x)}=0+2x+2=
\\f'_{(x)}=2+2x=2(x+1)