\\4) f_{(x)}=\dfrac{x-2}{x+3}=
\\\\f'_{(x)}=\lim_{\Delta x\rightarrow 0}\dfrac{\dfrac{(x+\Delta x)-2}{(x+\Delta x)+3}-\dfrac{x-2}{x+3}}{\Delta x}=
\\\\f'_{(x)}=\lim_{\Delta x\rightarrow 0}\dfrac{\dfrac{(x+\Delta x-2)(x+3)-(x-2)(x+\Delta x+3)}{(x+\Delta x+3)(x+3)}}{\Delta x}=
\\\\f'_{(x)}=\lim_{\Delta x\rightarrow 0}\dfrac{\dfrac{(x+\Delta x-2)(x+3)-(x-2)(x+\Delta x+3)}{(x+\Delta x+3)(x+3)}}{\Delta x}=
\\\\f'_{(x)}=\lim_{\Delta x\rightarrow 0}\dfrac{(x^2+x\Delta x-2x+3x+3\Delta x-6)-(x^2-2x+x\Delta x-2\Delta x+3x-6)}{\Delta x(x+\Delta x+3)(x+3)}=
\\\\f'_{(x)}=\lim_{\Delta x\rightarrow 0}\dfrac{\cancel{x^2}+\cancel{x\Delta x}+\cancel x+3\Delta x\cancel{-6}\cancel{-x^2}\cancel{-x\Delta x}+2\Delta x\cancel{-x}+\cancel6}{\Delta x(x+\Delta x+3)(x+3)}=
\\\\f'_{(x)}=\lim_{\Delta x\rightarrow 0}\dfrac{5\cancel{\Delta x}}{\cancel{\Delta x}(x+\Delta x+3)(x+3)}=
\\\\f'_{(x)}=\lim_{\Delta x\rightarrow 0}\dfrac{5}{(x+\Delta x+3)(x+3)}=
\\\\f'_{(x)}=\dfrac{5}{(x+\cancel 0+3)(x+3)}=
\\\\f'_{(x)}=\dfrac{5}{(x+3)^2}