\\52)f_{(x)}=\left(\dfrac{x^3+x}{x-1}\right)^{15}
\\\\f'_{(x)}=\left(\left(\dfrac{x^3+x}{x-1}\right)^{15}\right)'
\\\\f'_{(x)}=15\left(\dfrac{x^3+x}{x-1}\right)^{14}\left(\dfrac{(x^3+x)'(x-1)-(x^3+x)(x-1)'}{(x-1)^2}\right)
\\\\f'_{(x)}=15\left(\dfrac{x^3+x}{x-1}\right)^{14}\left(\dfrac{((x^3)'+x')(x-1)-(x^3+x)\cancel{(x'-\cancel{1'})}}{(x-1)^2}\right)
\\\\f'_{(x)}=15\left(\dfrac{x^3+x}{x-1}\right)^{14}\left(\dfrac{(3x^2+1)(x-1)-(x^3+x)}{(x-1)^2}\right)
\\\\f'_{(x)}=15\left(\dfrac{x^3+x}{x-1}\right)^{14}\left(\dfrac{3x^3+\cancel x-3x^2-1-x^3-\cancel x}{(x-1)^2}\right)
\\\\f'_{(x)}=15\left(\dfrac{x^3+x}{x-1}\right)^{14}\left(\dfrac{2x^3-3x^2-1}{(x-1)^2}\right)
