\\3) f(x)=\left(\dfrac{3x^3-2x}{x^2+3}\right)^{30}
\\\\f'(x)=30\left(\dfrac{3x^3-2x}{x^2+3}\right)^{29}\left(\dfrac{3x^3-2x}{x^2+3}\right)'
\\\\f'(x)=30\left(\dfrac{3x^3-2x}{x^2+3}\right)^{29}\dfrac{(3x^3-2x)'(x^2+3)-(3x^3-2x)(x^2+3)'}{(x^2+3)^2}
\\\\f'(x)=30\left(\dfrac{3x^3-2x}{x^2+3}\right)^{29}\dfrac{((3x^3)'-2\cancel{x'})(x^2+3)-(3x^3-2x)((x^2)'+\cancel{3'})}{(x^2+3)^2}
\\\\f'(x)=30\left(\dfrac{3x^3-2x}{x^2+3}\right)^{29}\dfrac{(9x^2-2)(x^2+3)-2x(3x^3-2x)}{(x^2+3)^2}
\\\\f'(x)=\dfrac{30(3x^3-2x)^{29}(9x^4-2x^2+27x^2-6-6x^4+4x^2)}{(x^2+3)^{29}(x^2+3)^2}
\\\\f'(x)=\dfrac{30x^{29}(3x^2-2)^{29}(3x^4+29x^2-6)}{(x^2+3)^{31}}