\\4)f(x)=\dfrac{\ln{(x^4-3x)}}{x^3+2}
\\\\f'(x)=\dfrac{\ln{(x^4-3x)}'(x^3+2)-\ln{(x^4-3x)}(x^3+2)'}{(x^3+2)^2}
\\\\f'(x)=\dfrac{\dfrac{x^3+2}{x^4-3x}-\ln{(x^4-3x)}((x^3)'+\cancel{2'})}{(x^3+2)^2}
\\\\f'(x)=\dfrac{\dfrac{x^3+2}{x^4-3x}-3x^2\ln{(x^4-3x)}}{(x^3+2)^2}
\\\\f'(x)=\dfrac{\dfrac{x^3+2-(x^4-3x)3x^2\ln{(x^4-3x)}}{x^4-3x}}{(x^3+2)^2}
\\\\f'(x)=\dfrac{x^3+2-3x^6\ln{(x^4-3x)}+9x^3\ln{(x^4-3x)}}{(x^6+4x^3+4)(x^4-3x)}
\\\\f'(x)=\dfrac{x^3+2-3x^3(x^3\ln{(x^4-3x)}-3\ln{(x^4-3x)})}{x^{10}+4x^7+4x^4-3x^7-12x^4-12x}
\\\\f'(x)=\dfrac{x^3+2-3x^3(x^3\ln{(x^4-3x)}-3\ln{(x^4-3x)})}{x(x^9+x^6-8x^3-12)}