\\3) f_{(x)}=\sqrt x
\\f'_{(x)}=\lim_{\Delta x\rightarrow 0}\dfrac{\sqrt{x + \Delta x}-\sqrt x}{\Delta x}\cdot\dfrac{\sqrt{x + \Delta x}+\sqrt x}{\sqrt{x + \Delta x}+\sqrt x}=
\\f'_{(x)}=\lim_{\Delta x\rightarrow 0}\dfrac{\sqrt{x + \Delta x}^2-\sqrt x^2}{\Delta x(\sqrt{x + \Delta x}+\sqrt x)}=
\\f'_{(x)}=\lim_{\Delta x\rightarrow 0}\dfrac{\cancel x + \Delta x\cancel{-x}}{\Delta x(\sqrt{x + \Delta x}+\sqrt x)}=
\\f'_{(x)}=\dfrac{\cancel{\Delta x}}{\cancel{\Delta x}(\sqrt{x + \Delta x}+\sqrt x)}=
\\f'_{(x)}=\dfrac{1}{\sqrt{x + \cancel 0}+\sqrt x}=
\\f'_{(x)}=\dfrac{1}{2\sqrt{x}}