\\5) f_{(x)}=\dfrac{3}{x+1}
\\\\f'_{(x)}=\lim_{\Delta x\rightarrow 0}\dfrac{\dfrac{3}{(x+\Delta x)+1}-\dfrac{3}{x+1}}{\Delta x}=
\\\\f'_{(x)}=\lim_{\Delta x\rightarrow 0}\dfrac{\dfrac{3(x+1)-3(x+\Delta x+1)}{(x+\Delta x+1)(x+1)}}{\Delta x}=
\\\\f'_{(x)}=\lim_{\Delta x\rightarrow 0}\dfrac{(3x+3)-(3x+3\Delta x+3)}{\Delta x(x+\Delta x+1)(x+1)}=
\\\\f'_{(x)}=\lim_{\Delta x\rightarrow 0}\dfrac{\cancel{3x}\cancel{+3}\cancel{-3x}-3\Delta x\cancel{-3}}{\Delta x(x+\Delta x+1)(x+1)}=
\\\\f'_{(x)}=\lim_{\Delta x\rightarrow 0}\dfrac{-3\cancel{\Delta x}}{\cancel{\Delta x}(x+\Delta x+1)(x+1)}=
\\\\f'_{(x)}=\dfrac{-3}{(x+\cancel 0+1)(x+1)}=
\\\\f'_{(x)}=-\dfrac{3}{(x+1)^2}