\\2)f_{(x)}=\dfrac{2}{x^2+5}=
\\\\f'_{(x)}=\lim_{\Delta x\rightarrow 0}\dfrac{\dfrac{2}{(x+\Delta x)^2+5}-\dfrac{2}{x^2+5}}{\Delta x}=
\\\\f'_{(x)}=\lim_{\Delta x\rightarrow 0}\dfrac{\dfrac{2}{x^2+2x\Delta x+\Delta x^2+5}-\dfrac{2}{x^2+5}}{\Delta x}=
\\\\f'_{(x)}=\lim_{\Delta x\rightarrow 0}\dfrac{\dfrac{2(x^2+5)-2(x^2+2x\Delta x+\Delta x^2+5)}{(x^2+2x\Delta x+\Delta x^2+5)(x^2+5)}}{\Delta x}=
\\\\f'_{(x)}=\lim_{\Delta x\rightarrow 0}\dfrac{2(x^2+5)-2(x^2+2x\Delta x+\Delta x^2+5)}{\Delta x(x^2+2x\Delta x+\Delta x^2+5)(x^2+5)}=
\\\\f'_{(x)}=\lim_{\Delta x\rightarrow 0}\dfrac{\cancel{2x^2}\cancel{+10}\cancel{-2x^2}-4x\Delta x-2\Delta x^2\cancel{-10}}{\Delta x(x^2+2x\Delta x+\Delta x^2+5)(x^2+5)}=
\\\\f'_{(x)}=\lim_{\Delta x\rightarrow 0}\dfrac{-2\cancel{\Delta x}(2+\Delta x)}{\cancel{\Delta x}(x^2+2x\Delta x+\Delta x^2+5)(x^2+5)}=
\\\\f'_{(x)}=\dfrac{-2(2+\cancel0)}{(x^2+\cancel{2x\cdot0}+\cancel{0^2}+5)(x^2+5)}=
\\\\f'_{(x)}=\dfrac{-4x}{(x^2+5)^2}=-\dfrac{4x}{(x^2+5)}=-\left(\dfrac{2x}{x^2-5}\right)^2