\\7)f_{(x)}=\sqrt{x^2-2x+3}
\\\\f'_{(x)}=\lim_{\Delta x\rightarrow0}\dfrac{\sqrt{(x+\Delta x)^2-2(x+\Delta x)+3}-\sqrt{x^2-2x+3}}{\Delta x}\cdot\left(\dfrac{\sqrt{(x+\Delta x)^2-2(x+\Delta x)+3}+\sqrt{x^2-2x+3}}{\sqrt{(x+\Delta x)^2-2(x+\Delta x)+3}+\sqrt{x^2-2x+3}}\right)
\\\\f'_{(x)}=\lim_{\Delta x\rightarrow0}\dfrac{\sqrt{x^2+2x\Delta x+\Delta x^2-2x-2\Delta x+3}^2-\sqrt{x^2-2x+3}^2}{\Delta x(\sqrt{(x+\Delta x)^2-2(x+\Delta x)+3}+\sqrt{x^2-2x+3})}
\\\\f'_{(x)}=\lim_{\Delta x\rightarrow0}\dfrac{\cancel{x^2}+2x\Delta x+\Delta x^2\cancel{-2x}-2\Delta x\cancel{+3}\cancel{-x^2}\cancel{+2x}\cancel{-3}}{\Delta x(\sqrt{(x+\Delta x)^2-2(x+\Delta x)+3}+\sqrt{x^2-2x+3})}
\\\\f'_{(x)}=\lim_{\Delta x\rightarrow0}\dfrac{\cancel{x^2}+2x\Delta x+\Delta x^2\cancel{-2x}-2\Delta x\cancel{+3}\cancel{-x^2}\cancel{+2x}\cancel{-3}}{\Delta x(\sqrt{(x+\Delta x)^2-2(x+\Delta x)+3}+\sqrt{x^2-2x+3})}
\\\\f'_{(x)}=\lim_{\Delta x\rightarrow0}\dfrac{\cancel{\Delta x}(2x+\Delta x-2)}{\cancel{\Delta x}(\sqrt{(x+\Delta x)^2-2(x+\Delta x)+3}+\sqrt{x^2-2x+3})}
\\\\f'_{(x)}=\dfrac{2x+\cancel0-2}{\sqrt{(x+\cancel0)^2-2(x+\cancel0)+3}+\sqrt{x^2-2x+3}}
\\\\f'_{(x)}=\dfrac{\cancel2(x-1)}{\cancel2\sqrt{x^2-2x+3}}
\\\\f'_{(x)}=\dfrac{x-1}{\sqrt{x^2-2x+3}}