\\9)f_{(x)}=\dfrac{x-1}{x^2+3x}
\\\\f'_{(x)}=\lim_{\Delta x\rightarrow0}\dfrac{\dfrac{x+\Delta x-1}{(x+\Delta x)^2+3x}-\dfrac{x-1}{x^2+3x}}{\Delta x}
\\\\f'_{(x)}=\lim_{\Delta x\rightarrow0}\dfrac{\dfrac{x+\Delta x-1}{x^2+2x\Delta x+\Delta x^2+3x}-\dfrac{x-1}{x^2+3x}}{\Delta x}
\\\\f'_{(x)}=\lim_{\Delta x\rightarrow0}\dfrac{\dfrac{(x+\Delta x-1)(x^2+3x)-(x-1)(x^2+2x\Delta x+\Delta x^2+3x)}{(x^2+2x\Delta x+\Delta x^2+3x)(x^2+3x)}}{\Delta x}
\\\\f'_{(x)}=\lim_{\Delta x\rightarrow0}\dfrac{\cancel{x^3}+x^2\Delta x\cancel{-x^2}\cancel{+3x^2}+3x\Delta x\cancel{-3x}\cancel{-x^3}-2x^2\Delta x-x\Delta x^2\cancel{-3x^2}+\cancel{x^2}+2x\Delta x+\Delta x^2\cancel{+3x}}{\Delta x(x^2+2x\Delta x+\Delta x^2+3x)(x^2+3x)}
\\\\f'_{(x)}=\lim_{\Delta x\rightarrow0}\dfrac{\cancel{\Delta x}(x^2+3x-2x^2-x\Delta x+2x+\Delta x)}{\cancel{\Delta x}(x^2+2x\Delta x+\Delta x^2+3x)(x^2+3x)}
\\\\f'_{(x)}=\dfrac{x^2+3x-2x^2-\cancel{x\cdot0}+2x+\cancel0}{(x^2+\cancel{2x\cdot0}+\cancel{0^2}+3x)(x^2+3x)}
\\\\f'_{(x)}=\dfrac{-x^2+5x}{(x^2+3x)^2}