\\1)f(x)=(4x^5-x)\ln{(2x^6+3x^4)}
\\\\f'(x)=(4x^5-x)'\ln{(2x^6+3x^4)}+(4x^5-x)\ln{(2x^6+3x^4)}'
\\\\f'(x)=((4x^5)'-x')\ln{(2x^6+3x^4)}+\dfrac{(4x^5-x)(2x^6+3x^4)'}{2x^6+3x^4}
\\\\f'(x)=(20x^4-1)\ln{(2x^6+3x^4)}+\dfrac{(4x^5-x)((2x^6)'+(3x^4)')}{2x^6+3x^4}
\\\\f'(x)=\dfrac{(2x^6+3x^4)(20x^4-1)\ln{(2x^6+3x^4)}+(4x^5-x)(12x^5+12x^3)}{2x^6+3x^4}
\\\\f'(x)=\dfrac{x^4(40x^6+60x^4-2x^2-3)\ln{(2x^6+3x^4)}+x^4(48x^6-12x^2+48x^4-12)}{x^4(2x^2+3)}
\\\\f'(x)=\dfrac{\cancel{x^4}((40x^6+60x^4-2x^2-3)\ln{(2x^6+3x^4)}+(48x^6-12x^2+48x^4-12))}{\cancel{x^4}(2x^2+3)}
\\\\f'(x)=\dfrac{(40x^6+60x^4-2x^2-3)\ln{(2x^6+3x^4)}+(48x^6-12x^2+48x^4-12)}{2x^2+3}